src/tactics/FStar.Tactics.Basic.fsi
@@ -65,7 +65,7 @@ val launch_process : string -> string -> string -> tac<string>
 val fresh_bv_named : string -> typ -> tac<bv>
 
 val pointwise : direction -> tac<unit> -> tac<unit>
-val topdown_rewrite: tac<(bool * FStar.BigInt.t)> -> tac<unit>
+val topdown_rewrite: (term -> tac<(bool * FStar.BigInt.t)>) -> tac<unit> -> tac<unit>
 val trefl : tac<unit>
 
 val dup : tac<unit>
