ulib/FStar.Tactics.Builtins.fst
@@ -218,8 +218,11 @@ what to do (to not do anything, use [trefl]). *)
 let pointwise  (tau : unit -> Tac unit) : Tac unit = TAC?.reflect (__pointwise BottomUp (reify (tau ())))
 let pointwise' (tau : unit -> Tac unit) : Tac unit = TAC?.reflect (__pointwise TopDown  (reify (tau ())))
 
-assume private val __topdown_rewrite : __tac (bool * int) -> __tac unit
-let topdown_rewrite (tau : unit -> Tac (bool * int)) : Tac unit = TAC?.reflect (__topdown_rewrite (reify (tau ())))
+assume private val __topdown_rewrite : (term -> __tac (bool * int)) -> __tac unit -> __tac unit
+let topdown_rewrite (ctrl : term -> Tac (bool * int)) (rw:unit -> Tac unit) : Tac unit =
+  TAC?.reflect (__topdown_rewrite
+                   (fun x -> reify (ctrl x))
+                   (reify (rw ())))
 
 assume private val __later : __tac unit
 (** Push the current goal to the back. *)
